Reorganize codebase into Lib/ and Examples/

src/Examples/Tree/Tree.v
@@ -1,72 +1,4 @@
-Require Import Coq.ZArith.ZArith.
-Require Import bedrock2.Syntax.
-Require Import bedrock2.WeakestPreconditionProperties.
-Require Import bedrock2.Map.Separation.
-Require Import bedrock2.Map.SeparationLogic.
-Require Import coqutil.Word.Interface coqutil.Word.Properties.
-Require Import coqutil.Map.Interface coqutil.Map.Properties.
-Ltac cleanup :=
-  repeat first [ progress cbn [fst snd eq_rect] in *
-               | match goal with H : _ /\ _ |- _ => destruct H end
-               | match goal with H : exists _, _ |- _ => destruct H end
-               | match goal with H : ?x = ?x |- _ => clear H end ].
-
-Ltac sepsimpl_step' :=
-  match goal with
-  | |- sep (emp _) _ _ => apply sep_emp_l
-  | |- sep _ (emp _) _ => apply sep_emp_r
-  | |- sep (fun m => emp _ m) _ _ => apply sep_emp_l
-  | |- sep _ (fun m => emp _ m) _ => apply sep_emp_r
-  | |- sep (Lift1Prop.ex1 _) _ _ => apply sep_ex1_l
-  | |- sep _ (Lift1Prop.ex1 _) _ => apply sep_ex1_r
-  | |- emp _ _ => split; [ congruence | ]
-  end.
-
-Ltac sepsimpl_step :=
-  match goal with
-  | _ => sepsimpl_step'
-  | |- sep (sep _ _) _ _ => apply sep_assoc; sepsimpl_step'
-  | |- sep _ (sep _ _) _ => apply sep_comm, sep_assoc; sepsimpl_step'
-  | |- sep _ _ _ => apply sep_comm; sepsimpl_step'
-  end.
-
-Ltac sepsimpl_in H :=
-  match type of H with
-  | sep (emp _) _ _ =>
-    eapply sep_emp_l in H
-  | sep _ (emp _) _ =>
-    eapply sep_emp_r in H
-  | sep (fun m => emp _ m) _ _ =>
-    eapply sep_emp_l in H
-  | sep _ (fun m => emp _ m) _ =>
-    eapply sep_emp_r in H
-  | sep (Lift1Prop.ex1 _) _ _ =>
-    eapply sep_ex1_l in H; destruct H
-  | sep _ (Lift1Prop.ex1 _) _ =>
-    eapply sep_ex1_r in H; destruct H
-  end.
-
-Ltac sepsimpl_hyps_step :=
-  match goal with
-  | H : False |- _ => tauto
-  | H : emp _ _ |- _ => cbv [emp] in H; destruct H
-  | H : Lift1Prop.ex1 _ _ |- _ => destruct H
-  | H : sep (sep ?p ?q) _ _ |- _ =>
-    eapply (sep_assoc p q) in H; sepsimpl_in H
-  | H : sep _ _ _ |- _ => sepsimpl_in H
-  | H : sep _ (sep ?p ?q) _ |- _ =>
-    eapply sep_comm, (sep_assoc p q) in H; sepsimpl_in H
-  end.
-
-Ltac sepsimpl_hyps :=
-  repeat first [ progress cleanup
-               | progress sepsimpl_hyps_step ].
-
-Ltac sepsimpl :=
-  repeat first [ progress cleanup
-               | match goal with |- _ /\ _ => split end
-               | progress sepsimpl_step
-               | progress sepsimpl_hyps_step ].
+Require Import Rupicola.Lib.Api.
 
 Section Tree.
   Context {p : Semantics.parameters}.
@@ -102,7 +34,7 @@ Section Tree.
       | Node _ l r => Node a l r
       end.
 
-    Fixpoint find
+    Fixpoint lookup
              (t : tree alpha)
              (cond : alpha -> bool)
       : option alpha :=
@@ -110,9 +42,9 @@ Section Tree.
       | Empty => None
       | Node a l r =>
         if cond a then Some a
-        else match find l cond with
+        else match lookup l cond with
              | Some a => Some a
-             | None => find r cond
+             | None => lookup r cond
              end
       end.
 
@@ -208,10 +140,10 @@ Section Tree.
       Local Notation Tree :=
         (@Tree _ Alpha word_size_in_bytes).
 
-      Lemma find_replace t cond :
+      Lemma lookup_replace t cond :
         forall a olda pt pa R mem,
           sep (sep (Tree pt t) (Alpha pa a)) R mem ->
-          find t cond = Some (Borrowed pa olda) ->
+          lookup t cond = Some (Borrowed pa olda) ->
           sep (Tree pt (fst (replace t cond (Owned a)))) R mem.
       Proof.
         induction t; intros;
