src/Examples/Cells/Cells.v
@@ -1,0 +1,97 @@
+Require Import Rupicola.Lib.Api.
+
+Record cell := { data : Semantics.word }.
+
+Definition cell_value (addr: address) (c: cell) : Semantics.mem -> Prop :=
+  scalar addr c.(data).
+
+Definition TwoCells a_ptr b_ptr ab : Semantics.mem -> Prop :=
+  sep (cell_value a_ptr (fst ab)) (cell_value b_ptr (snd ab)).
+
+Hint Unfold TwoCells : compiler.
+
+Definition get c := c.(data).
+Definition put v (c: cell) := {| data := v |}.
+
+Lemma compile_get :
+  forall (locals: Semantics.locals) (mem: Semantics.mem)
+    tr R R' functions T (pred: T -> _ -> Prop) c c_ptr c_var k k_impl,
+  forall var,
+    sep (cell_value c_ptr c) R' mem ->
+    map.get locals c_var = Some c_ptr ->
+    let v := (get c) in
+    (let head := v in
+     find k_impl
+     implementing (pred (k head))
+     with-locals (map.put locals var head)
+     and-memory mem and-trace tr and-rest R
+     and-functions functions) ->
+    (let head := v in
+     find (cmd.seq (cmd.set var (expr.load access_size.word (expr.var c_var)))
+                   k_impl)
+     implementing (pred (dlet head k))
+     with-locals locals and-memory mem and-trace tr and-rest R
+     and-functions functions).
+Proof.
+  intros.
+  repeat straightline.
+  exists (get c).
+  split.
+  { cbn.
+    red.
+    exists c_ptr.
+    split.
+    { eassumption. }
+    { eexists; split; [ | reflexivity ].
+      eapply load_word_of_sep.
+      eassumption. } }
+  red; intros.
+  eassumption.
+Qed.
+
+Lemma compile_put :
+  forall (locals: Semantics.locals) (mem: Semantics.mem)
+    tr R R' functions T (pred: T -> _ -> Prop) c c_ptr c_var x x_var k k_impl,
+    sep (cell_value c_ptr c) R' mem ->
+    map.get locals c_var = Some c_ptr ->
+    map.get locals x_var = Some x ->
+    let v := (put x c) in
+    (let head := v in
+     forall m,
+       sep (cell_value c_ptr head) R' m ->
+       (find k_impl
+        implementing (pred (k head))
+        with-locals locals
+        and-memory m and-trace tr and-rest R
+        and-functions functions)) ->
+    (let head := v in
+     find (cmd.seq (cmd.store access_size.word (expr.var c_var) (expr.var x_var))
+                   k_impl)
+     implementing (pred (dlet head k))
+     with-locals locals and-memory mem and-trace tr and-rest R
+     and-functions functions).
+Proof.
+  intros.
+  unfold cell_value in *.
+  repeat straightline.
+  exists c_ptr.
+  split.
+  { repeat straightline; eauto. }
+  { eexists; split.
+    { repeat straightline; eauto. }
+    repeat straightline.
+    subst v; simpl.
+    match goal with
+    | [ H: context[WeakestPrecondition.cmd] |- _ ] => apply H
+    end.
+    eassumption. }
+Qed.
+
+Ltac cell_compile_step :=
+  gen_sym_inc;
+  let name := gen_sym_fetch "v" in
+  first [simple eapply compile_get with (var := name) |
+         simple eapply compile_put].
+
+Ltac compile_custom ::=
+  cell_compile_step.
