src/Examples/Cells/Incr.v
@@ -1,0 +1,25 @@
+Require Import Rupicola.Lib.Api.
+Require Import Rupicola.Examples.Cells.Cells.
+
+Definition incr_gallina_spec (c: cell) :=
+  let/d v := get c in
+  let/d one := word.of_Z 1 in
+  let/d v := word.add v one in
+  let/d c := put v c in
+  c.
+
+Derive body SuchThat
+       (let swap := ("swap", (["c"], [], body)) in
+        program_logic_goal_for swap
+        (forall functions,
+         forall c_ptr c tr R mem,
+           seps [cell_value c_ptr c; R] mem ->
+           WeakestPrecondition.call
+             (swap :: functions)
+             "swap"
+             tr mem [c_ptr]
+             (postcondition_for (cell_value c_ptr (incr_gallina_spec c)) R tr)))
+  As body_correct.
+Proof.
+  compile.
+Qed.
