src/Examples/Cells/Swap.v
@@ -1,0 +1,25 @@
+Require Import Rupicola.Lib.Api.
+Require Import Rupicola.Examples.Cells.Cells.
+
+Definition swap_gallina_spec (c1 c2: cell) :=
+  let/d v1 := get c1 in
+  let/d v2 := get c2 in
+  let/d c1 := put v2 c1 in
+  let/d c2 := put v1 c2 in
+  (c1, c2).
+
+Derive swap_body SuchThat
+       (let swap := ("swap", (["a"; "b"], [], swap_body)) in
+        program_logic_goal_for swap
+        (forall functions,
+         forall a_ptr a b_ptr b tr R mem,
+           sep (TwoCells a_ptr b_ptr (a,b)) R mem ->
+           WeakestPrecondition.call
+             (swap :: functions)
+             "swap"
+             tr mem [a_ptr;b_ptr]
+             (postcondition_for (TwoCells a_ptr b_ptr (swap_gallina_spec a b)) R tr)))
+  As swap_body_correct.
+Proof.
+  compile.
+Qed.
