src/Examples/KVStore/Automated.v
@@ -1,0 +1,583 @@
+Require Import Rupicola.Lib.Api.
+Require Import Rupicola.Examples.KVStore.KVStore.
+Require Import Rupicola.Examples.KVStore.Properties.
+Require Import Rupicola.Examples.KVStore.Tactics.
+
+Section KVSwap.
+  Context {ops} {key value : Type} {Value}
+          {dummy_value : value}
+          {kvp : kv_parameters}
+          {ok : @kv_parameters_ok ops key value Value kvp}.
+
+  Existing Instances ops kvp ok.
+  Existing Instances map_ok annotated_map_ok key_eq_dec.
+  Existing Instances spec_of_map_get.
+
+  (* MAP LAYOUTS
+
+
+  pk | key
+  pk+1 | pointer (pv)
+
+  pv | value
+
+  get v returns pk+1
+
+
+  Keys = words, inline
+  Values = ?? (pointers stored inline)
+
+  map = linked list of (key, value pointer) pairs
+
+  entry:
+
+  pk   | key1
+  pk+1 | value1
+  pk+2 | pk'
+  ...
+  pk'   | key2
+  pk'+1 | value2
+  pk'+2 | NULL
+
+  Value value1 tt
+  Value := fun (value : word) (x : unit) => emp True
+  get key1 --> value1 (and you now "own" value1, which means nothing)
+
+  put key1 value3 --> (1, value1) (and you now "own" value1, which means nothing)
+
+  pk   | key1
+  pk+1 | value3
+  pk+2 | pk'
+  ...
+  pk'   | key2
+  pk'+1 | value2
+  pk'+2 | NULL
+  ...
+  pk3 | key3
+
+  put key3 value4 --> (0, NULL)
+
+  pk   | key1
+  pk+1 | value3
+  pk+2 | pk'
+  ...
+  pk'   | key2
+  pk'+1 | value2
+  pk'+2 | pk3
+  ...
+  pk3 | key3
+
+
+
+  entry:
+
+  pk   | key1
+  pk+1 | pv1
+  pk+2 | pk'
+  ...
+  pv1 | value1
+  ...
+  pk'   | key2
+  pk'+1 | pv2
+  pk'+2 | NULL
+  ...
+  pv2 | value2
+
+  Value pv1 value1 * Value pv2 value2
+  Value := fun (addr x : word) => mem[addr] = x
+  Key := fun (addr : word) (x : unit) => emp True
+  get key1 --> pv1
+  get key2 --> pv2
+  borrow pv1
+  borrow pv2
+
+  pk   | key1
+  pk+1 | (pv1)
+  pk+2 | pk'
+  ...
+  pv1 | value1
+  ...
+  pk'   | key2
+  pk'+1 | (pv2)
+  pk'+2 | NULL
+  ...
+  pv2 | value2
+
+  put key1 pv2 (you own pv1 and pv2) --> 1 (map now owns pv2)
+
+  pk   | key1
+  pk+1 | pv2
+  pk+2 | pk'
+  ...
+  pv1 | value1
+  ...
+  pk'   | key2
+  pk'+1 | (pv2)
+  pk'+2 | NULL
+  ...
+  pv2 | value2
+
+  put key2 pv1 (you own pv1) --> 1 (map now owns pv1)
+
+  pk   | key1
+  pk+1 | pv2
+  pk+2 | pk'
+  ...
+  pv1 | value1
+  ...
+  pk'   | key2
+  pk'+1 | pv1
+  pk'+2 | NULL
+  ...
+  pv2 | value2
+
+   *)
+  Import KVStore.
+
+  Instance spec_of_map_put : spec_of put :=
+    fun functions =>
+      forall pm m pk k pv v R tr mem,
+        (AnnotatedMap pm m
+         * Key pk k * Value pv v * R)%sep mem ->
+        WeakestPrecondition.call
+          functions put tr mem [pm; pk; pv]
+          (fun tr' mem' rets =>
+             tr = tr'
+             /\ length rets = 0%nat
+             /\ match map.get m k with
+                | Some (Borrowed _, old_v) =>
+                  (AnnotatedMap pm (map.put m k (Owned, v))
+                   * Key pk k * R)%sep mem'
+                | _ =>
+                  (* not allowed! no guarantees for you *)
+                  True
+                end).
+
+
+  Definition do_or_default {A B}
+             (a : option A) (f : A -> B) (default : B) : B :=
+    match a with
+    | Some a => f a
+    | None => default
+    end.
+
+  Notation "'let/o'  x  :=  val  'goto_fail' default 'in'  body" :=
+    (do_or_default val (fun x => body) default) (at level 4).
+
+  (* look up k1 and k2, add their values and store in k3 *)
+  Definition kvswap_gallina (m : map.rep (map:=map))
+             (k1 k2 : key) : map.rep (map:=map) * key * key :=
+    let/o v1 := map.get m k1 goto_fail (m, k1, k2) in
+    let/o v2 := map.get m k2 goto_fail (m, k1, k2) in
+    let/d m := map.put m k2 v1 in
+    let/d m := map.put m k1 v2 in
+    (m, k1, k2).
+
+  (*
+  Definition swap : bedrock_func :=
+    let m := "m" in
+    let k1 := "k1" in
+    let k2 := "k2" in
+    let v1 := "v1" in
+    let v2 := "v2" in
+    let err := "err" in
+    ("swap",
+     ([m; k1; k2], [],
+      bedrock_func_body:(
+        unpack! err, v1 = get (m, k1) ;
+          require !err ;
+          unpack! err, v2 = get (m, k2) ;
+          require !err ;
+          unpack! err = put (m, k2, v1)
+          (* now v2 is stored in v1 -- no need for second put *)
+    ))).
+   *)
+
+  Definition MapAndTwoKeys pm pk1 pk2 v :=
+    let m := fst (fst v) in
+    let k1 := snd (fst v) in
+    let k2 := snd v in
+    (Map pm m * Key pk1 k1 * Key pk2 k2)%sep.
+
+  Definition deannotate (m : annotated_map) : map.rep (map:=map) :=
+    map.fold
+      (fun (m' : map.rep) (k : key) (v : annotation * value) =>
+         map.put m' k (snd v)) map.empty m.
+
+  Lemma get_deannotate_Some m k a v :
+    map.get m k = Some (a, v) ->
+    map.get (deannotate m) k = Some v.
+  Admitted.
+  Lemma get_deannotate_None m k :
+    map.get m k = None ->
+    map.get (deannotate m) k = None.
+  Admitted.
+
+  Definition is_owned {A} (an: annotation * A) :=
+    match an with
+    | (Owned, _) => True
+    | _ => False
+    end.
+  (* Arguments is_owned {A} / !an. *)
+
+  Definition is_borrowed {A} (an: annotation * A) :=
+    match an with
+    | (Borrowed _, _) => True
+    | _ => False
+    end.
+  (* Arguments is_borrowed {A} / !an. *)
+
+  Lemma get_annotate_is_Owned:
+    forall (m : map) (k1 : key) (a : annotation * value),
+      map.get (annotate m) k1 = Some a -> is_owned a.
+  Proof.
+    intros m k1 a H.
+    autorewrite with mapsimpl in H.
+    destruct_one_match_hyp.
+    - match goal with
+      | [ H: Some _ = Some _ |- _ ] => inversion H
+      end.
+      reflexivity.
+    - discriminate.
+  Qed.
+
+  Lemma compile_map_get :
+    forall (locals: Semantics.locals) (mem: Semantics.mem)
+           tr R R' functions T (pred: T -> _ -> Prop)
+           m m_ptr m_var M
+           k k_ptr k_var
+           default default_impl
+           K K_impl,
+      spec_of_map_get functions ->
+      m = deannotate M ->
+    forall err var,
+      var <> err ->
+      (AnnotatedMap m_ptr M * Key k_ptr k * R')%sep mem ->
+      map.get locals m_var = Some m_ptr ->
+      map.get locals k_var = Some k_ptr ->
+      (forall a, map.get M k = Some a -> is_owned a) ->
+      let v := (map.get m k) in
+      (forall garbage mem',
+          v = None ->
+          (AnnotatedMap m_ptr M * Key k_ptr k * R')%sep mem' ->
+          find default_impl
+          implementing (pred default)
+          with-locals (map.put (map.put locals err (word.of_Z 1))
+                            var garbage)
+          and-memory mem' and-trace tr and-rest R
+          and-functions functions) ->
+      (forall head hd_ptr mem',
+          v = Some head ->
+          (AnnotatedMap m_ptr
+                        (map.put M k
+                                 (Reserved hd_ptr, head))
+           * Key k_ptr k * R')%sep mem' ->
+          find K_impl
+          implementing (pred (K head))
+          with-locals (map.put (map.put locals err (word.of_Z 0))
+                            var hd_ptr)
+          and-memory mem' and-trace tr and-rest R
+          and-functions functions) ->
+      (let head := v in
+       find (cmd.seq
+               (cmd.call [err; var] (fst (@KVStore.get ops)) [expr.var m_var; expr.var k_var])
+               (cmd.cond (expr.op bopname.eq (expr.var err) (expr.literal 0))
+                         K_impl
+                         default_impl))
+       implementing (pred (do_or_default head K default))
+       with-locals locals and-memory mem and-trace tr and-rest R
+       and-functions functions).
+  Proof.
+    intros.
+    repeat straightline.
+    exists [m_ptr; k_ptr].
+    split.
+    { cbn.
+      eexists; split; [ eassumption | ].
+      eexists; split; [ eassumption | ].
+      reflexivity. }
+    kv_hammer.
+    destruct_one_match_hyp_of_type (option (annotation * value)).
+    { destruct_products.
+      destruct_one_match_hyp_of_type annotation;
+        match goal with
+        | [ H: forall a, Some _ = Some a -> _ |- _ ] => specialize (H _ eq_refl); cbn in H
+        end; try contradiction.
+      subst. subst m. subst v.
+      match goal with
+      | l := context [map.put _ err] |- _ => subst l
+      end.
+      erewrite get_deannotate_Some by eassumption.
+      cbn [do_or_default].
+      exists (word.of_Z 1).
+      split.
+      { eexists.
+        split.
+        { rewrite ?map.get_put_diff, map.get_put_same by congruence.
+          reflexivity. }
+        { reflexivity. } }
+      { rewrite word.unsigned_of_Z_1.
+        split; try congruence; [ ]. intros.
+        cbn [fst snd].
+        match goal with
+        | H : _ |- _ => apply H
+        end.
+        { erewrite get_deannotate_Some by eassumption.
+          reflexivity. }
+        { ecancel_assumption. } } }
+    { destruct_products.
+      subst. subst m. subst v.
+      match goal with
+      | l := context [map.put _ err] |- _ => subst l
+      end.
+      erewrite get_deannotate_None by eassumption.
+      cbn [do_or_default].
+      exists (word.of_Z 0).
+      split.
+      { eexists.
+        split.
+        { rewrite ?map.get_put_diff, map.get_put_same by congruence.
+          reflexivity. }
+        { reflexivity. } }
+      { rewrite word.unsigned_of_Z_0.
+        split; try congruence; [ ]. intros.
+        cbn [fst snd].
+        match goal with
+        | H : _ |- _ => apply H
+        end.
+        { eapply get_deannotate_None. eassumption. }
+        { ecancel_assumption. } } }
+  Qed.
+
+  (*
+  Instance spec_of_map_put : spec_of put :=
+    fun functions =>
+      forall pm m pk k pv v R tr mem,
+        (AnnotatedMap pm m
+         * Key pk k * Value pv v * R)%sep mem ->
+        WeakestPrecondition.call
+          functions put tr mem [pm; pk; pv]
+          (fun tr' mem' rets =>
+             tr = tr'
+             /\ length rets = 2%nat
+             /\ let was_overwrite := hd (word.of_Z 0) rets in
+               let old_ptr := hd (word.of_Z 0) (tl rets) in
+               match map.get m k with
+               | Some (a, old_v) =>
+                 match a with
+                 | Borrowed _ => True (* no guarantees *)
+                 | Reserved pv' =>
+                   was_overwrite = word.of_Z 1
+                   /\ old_ptr = pv'
+                   /\ (AnnotatedMap pm (map.put m k (Reserved pv, v))
+                      * Key pk k * Value old_ptr old_v * R)%sep mem'
+                 | Owned =>
+                   was_overwrite = word.of_Z 1
+                   /\ (AnnotatedMap pm (map.put m k (Owned, v))
+                      * Key pk k * Value old_ptr old_v * R)%sep mem'
+                 end
+               | None =>
+                 (* if there was no previous value, the map consumes both
+                     the key and value memory *)
+                 was_overwrite = word.of_Z 0
+                 /\ (AnnotatedMap pm (map.put m k (Owned, v))
+                    * R)%sep mem'
+               end).
+   *)
+
+  Lemma compile_map_put_replace :
+    forall (locals: Semantics.locals) (mem: Semantics.mem)
+           tr R R' functions T (pred: T -> _ -> Prop)
+           m m_ptr m_var M
+           k k_ptr k_var
+           v v_ptr v_var
+           K K_impl,
+      spec_of_map_put functions ->
+      m = deannotate M ->
+      (AnnotatedMap m_ptr M * Key k_ptr k * Value v_ptr v * R')%sep mem ->
+      map.get locals m_var = Some m_ptr ->
+      map.get locals k_var = Some k_ptr ->
+      map.get locals v_var = Some v_ptr ->
+      (exists a, map.get M k = Some a /\ is_borrowed a) ->
+      let m := (map.put m k v) in (* FIXME this should say put_replace *)
+      (forall mem',
+         let head := m in
+         (AnnotatedMap m_ptr (map.put M k (Owned, v))
+          * Key k_ptr k * R')%sep mem' ->
+         find K_impl
+         implementing (pred (K head))
+         with-locals locals
+         and-memory mem' and-trace tr and-rest R
+         and-functions functions) ->
+      (let head := m in
+       find (cmd.seq
+               (cmd.call []
+                         (fst (@KVStore.put ops))
+                         [expr.var m_var; expr.var k_var; expr.var v_var])
+               K_impl)
+       implementing (pred (dlet head K))
+       with-locals locals and-memory mem and-trace tr and-rest R
+       and-functions functions).
+  Proof.
+    intros.
+    repeat straightline.
+    exists [m_ptr; k_ptr; v_ptr].
+    split.
+    { cbn.
+      eexists; split; eauto.
+      eexists; split; eauto.
+      eexists; split; eauto. }
+    { kv_hammer.
+      match goal with
+      | [ H: forall mem, _ mem -> _ |- _ ] => apply H
+      end.
+      destruct_one_match_hyp_of_type annotation; try contradiction.
+      eassumption. }
+  Qed.
+
+  Hint Resolve get_annotate_is_Owned : compiler.
+
+  Lemma deannotate_annotate:
+    forall m : map, m = deannotate (annotate m).
+  Proof.
+  Admitted.
+
+  Hint Extern 1 (?m = deannotate (annotate ?m)) => simple apply deannotate_annotate : compiler.
+
+  Lemma get_deannotate_annotate:
+    forall k v (m : map),
+      map.get m k = v ->
+      map.get (deannotate (annotate m)) k = v.
+  Proof.
+    intros. rewrite <- deannotate_annotate; eauto.
+  Qed.
+
+  Hint Resolve get_deannotate_annotate : compiler.
+  Hint Unfold MapAndTwoKeys : compiler.
+
+  Lemma deannotate_put:
+    forall (m : map) M (k : key) (p : annotation * value),
+      m = map.put (deannotate M) k (snd p) ->
+      m = deannotate (map.put M k p).
+  Proof.
+  Admitted.
+
+  Hint Resolve deannotate_put : compiler.
+
+  Hint Extern 1 => simple eapply put_noop' : compiler.
+
+
+  Axiom __magic__ : forall {A}, A.
+  Ltac admitt := exfalso; clear; apply __magic__.
+
+  Derive kvswap_body SuchThat
+         (let kvswap := ("kvswap", (["m"; "k1"; "k2"], [],
+                                    kvswap_body)) in
+          program_logic_goal_for kvswap
+          (forall functions,
+              spec_of_map_get functions ->
+              spec_of_map_put functions ->
+              forall pm m pk1 k1 pk2 k2 R tr mem,
+                k1 <> k2 -> (* TODO: try removing *)
+                (Map pm m * Key pk1 k1 * Key pk2 k2 * R)%sep mem ->
+                WeakestPrecondition.call
+                  (kvswap :: functions)
+                  "kvswap"
+                  tr mem [pm; pk1; pk2]
+                  (postcondition_for
+                     (MapAndTwoKeys
+                        pm pk1 pk2
+                        (kvswap_gallina m k1 k2)) R tr)))
+      As kvswap_body_correct.
+  Proof.
+    setup.
+    (* Is there a systematic way to move from unannotated to annotated? The
+    annotated spec is better for composing definitions, but the unannotated
+    one is better for reading specs. *)
+    add_map_annotations.
+    eapply compile_map_get with (var:="v1") (err:="err") (M:=annotate m).
+    all: repeat compile_step; eauto with compiler.
+    { match goal with
+      | [  |- _ <> _ ] => congruence
+      end. }
+    { intros.               (* FIXME compile_step *)
+      clear_old_seps.
+      compile_step.
+      autounfold with compiler.
+      cbn [fst snd].
+      remove_map_annotations. (* FIXME *)
+      compile_step. }
+    { intros.
+      clear_old_seps.
+      eapply compile_map_get with (var:="v2") (err:="err"); repeat compile_step.
+      { eauto with compiler. }
+      { match goal with
+        | [  |- _ <> _ ] => congruence
+        end. }
+      { intros.
+        Hint Rewrite @map.get_put_diff @map.get_put_same @map.put_put_same
+             @annotate_get_Some @annotate_get_None
+             using (typeclasses eauto || congruence) : mapsimpl_not_too_much.
+
+        autorewrite with mapsimpl_not_too_much in *. (* FIXME is that enough for the other cases? *)
+        eauto with compiler. }
+      { intros.
+        clear_old_seps.
+        repeat compile_step.
+        remove_map_annotations. (* Should be done only in the skip case *)
+        repeat compile_step. }
+      { intros; clear_old_seps.
+        repeat compile_step.
+        eapply compile_map_put_replace;
+          lazymatch goal with
+          | [  |- sep _ _ _ ] => borrow_all
+          | _ => idtac
+          end.
+        3: ecancel_assumption.
+        all: repeat compile_step; eauto with compiler.
+        { Print HintDb compiler.
+          simple apply deannotate_put.
+          cbn.
+          eapply put_noop';
+            eauto 10 with compiler.
+          autorewrite with mapsimpl_not_too_much.
+          admitt.
+        }
+        all: eauto.
+        { repeat match goal with
+                 | [  |- exists _, _ ] => eexists
+                 | [  |- _ /\ _ ] => split
+                 | _ => progress autorewrite with mapsimpl_not_too_much
+                 | _ => reflexivity
+                 end. }
+        intros.
+        clear_old_seps.
+
+        (* autorewrite with mapsimpl. *)
+        (* rewrite map.put_put_same in H3. *)
+
+        eapply compile_map_put_replace;
+          lazymatch goal with
+          | [  |- sep _ _ _ ] => try borrow_all
+          | _ => idtac
+          end.
+
+        all: repeat compile_step; eauto with compiler.
+
+        all: subst head1.
+        { apply map.map_ext.
+          intros; autorewrite with mapsimpl.
+          admitt. }
+          { repeat match goal with
+                 | [  |- exists _, _ ] => eexists
+                 | [  |- _ /\ _ ] => split
+                 | _ => progress autorewrite with mapsimpl_not_too_much
+                 | _ => reflexivity
+                      end. }
+        { intros.
+          clear_old_seps.
+          repeat compile_step.
+          remove_map_annotations. (* Should be done only in the skip case *)
+          repeat compile_step. }
+  Abort.
+End KVSwap.
