src/Examples/Ttl/Ttl.v
@@ -1,33 +1,10 @@
-Require Import Coq.ZArith.ZArith.
-Require Import Coq.Strings.String.
-Require Import Coq.Lists.List.
-Require Import Coq.micromega.Lia.
-Require Import bedrock2.Array.
-Require Import bedrock2.BasicCSyntax.
-Require Import bedrock2.BasicC64Semantics.
-Require Import bedrock2.ProgramLogic.
-Require Import bedrock2.Scalars.
-Require Import bedrock2.Syntax.
-Require Import bedrock2.WeakestPreconditionProperties.
-Require Import bedrock2.Map.Separation.
-Require Import bedrock2.Map.SeparationLogic.
-Require Import coqutil.Word.Interface coqutil.Word.Properties.
-Require Import coqutil.Map.Interface coqutil.Map.Properties.
-Require Import coqutil.Map.SortedList.
-Require Import coqutil.Tactics.destr.
-Require Import coqutil.Tactics.Tactics.
-Require Import Coq.Numbers.DecimalString.
+Require Import Rupicola.Lib.Api.
 
-Local Open Scope string_scope.
-Import ListNotations.
+Local Notation function_t :=
+  ((String.string * (list String.string * list String.string * Syntax.cmd.cmd))%type).
+Local Notation functions_t :=
+  (list function_t).
 
-Require Import Incr.
-Import GallinaIncr.
-Import dlet.
-
-
-Local Notation function_t := ((String.string * (list String.string * list String.string * Syntax.cmd.cmd))%type).
-Local Notation functions_t := (list function_t).
 (* modified version of program_logic_goal_for_function, in which callee names
   are manually inserted *)
 Ltac program_logic_goal_for_function proc callees :=
@@ -41,216 +18,204 @@ Ltac program_logic_goal_for_function proc callees :=
                               (spec (cons proc functions)) in
                    exact s)).
 
-Module Ttl.
-  Local Existing Instance bedrock2.BasicCSyntax.StringNames_params.
-  Local Existing Instance BasicC64Semantics.parameters.
-  Local Existing Instance BasicC64Semantics.parameters_ok.
+(* Definition packet := *)
+(*   hlist.t ["field1"; …; "ttl"] [Semantics.byte; …; Semantics.byte]. (* field1, ttl *) *)
 
-  (* FIXME update bedrock2 to get rid of Semantics.byte *)
-  (* Definition packet := *)
-  (*   hlist.t ["field1"; …; "ttl"] [Semantics.byte; …; Semantics.byte]. (* field1, ttl *) *)
+Definition packet :=
+  Vector.t Semantics.word 2. (* field1, ttl *)
 
-  Definition packet :=
-    Vector.t Semantics.word 2. (* field1, ttl *)
+Local Declare Scope sep_scope.
+Local Delimit Scope sep_scope with sep.
+Local Infix "*" := (sep) : sep_scope.
 
-  Local Declare Scope sep_scope.
-  Local Delimit Scope sep_scope with sep.
-  Local Infix "*" := (sep) : sep_scope.
+Notation address := Semantics.word.
 
-  Notation address := Semantics.word.
+Notation field1_index := Fin.F1.
+Notation ttl_index := (Fin.FS Fin.F1).
+Notation field1 p := (Vector.nth p field1_index).
+Notation ttl p := (Vector.nth p ttl_index).
 
-  Notation field1_index := Fin.F1.
-  Notation ttl_index := (Fin.FS Fin.F1).
-  Notation field1 p := (Vector.nth p field1_index).
-  Notation ttl p := (Vector.nth p ttl_index).
+Definition WordVector {n} (addr: address) (v: Vector.t Semantics.word n) : Semantics.mem -> Prop :=
+  array scalar (word.of_Z 8) addr (Vector.to_list v).
 
-  Definition WordVector {n} (addr: address) (v: Vector.t Semantics.word n) : Semantics.mem -> Prop :=
-    array scalar (word.of_Z 8) addr (Vector.to_list v).
+Definition Packet (addr: address) (p: packet) : Semantics.mem -> Prop :=
+  WordVector addr p.
 
-  Definition Packet (addr: address) (p: packet) : Semantics.mem -> Prop :=
-    WordVector addr p.
+Definition decr_gallina (p: packet) :=
+  let/d ttl := (ttl p) in
+  let/d m1 := word.of_Z (-1) in
+  let/d ttl := word.add ttl m1 in
+  let/d p := Vector.replace p ttl_index ttl in
+  p.
 
-  Definition decr_gallina (p: packet) :=
-    let/d ttl := (ttl p) in
-    let/d m1 := word.of_Z (-1) in
-    let/d ttl := word.add ttl m1 in
-    let/d p := Vector.replace p ttl_index ttl in
-    p.
+Lemma vector_uncons {A n} (v: Vector.t A n) :
+  match n return Vector.t A n -> Prop with
+  | 0 => fun v => v = Vector.nil _
+  | S n =>fun v => v = Vector.cons _ (Vector.hd v) _ (Vector.tl v)
+  end v.
+Proof.
+  destruct v; reflexivity.
+Qed.
 
-  Import GallinaIncr.
+Lemma Vector_to_list_length {A n} (v: Vector.t A n):
+  Datatypes.length (Vector.to_list v) = n.
+Proof. Admitted.
 
-  Lemma vector_uncons {A n} (v: Vector.t A n) :
-    match n return Vector.t A n -> Prop with
-    | 0 => fun v => v = Vector.nil _
-    | S n =>fun v => v = Vector.cons _ (Vector.hd v) _ (Vector.tl v)
-    end v.
-  Proof.
-    destruct v; reflexivity.
-  Qed.
-
-  Lemma Vector_to_list_length {A n} (v: Vector.t A n):
-    Datatypes.length (Vector.to_list v) = n.
-  Proof. Admitted.
-
-  Lemma compile_nth :
-    forall (locals: Semantics.locals) (mem: Semantics.mem)
-      tr R R' functions T (pred: T -> _ -> Prop)
-      {n} (vector: Vector.t Semantics.word n) vector_ptr vector_var
-      offset var k k_impl,
-      (Z.of_nat n < 2 ^ Semantics.width)%Z ->
-      sep (WordVector vector_ptr vector) R' mem ->
-      map.get locals vector_var = Some vector_ptr ->
-      let v := Vector.nth vector offset in
-      let noffset := proj1_sig (Fin.to_nat offset) in
-      (let head := v in
-       forall m,
-         sep (WordVector vector_ptr vector) R' m ->
-         (find k_impl
-          implementing (pred (k head))
-          with-locals (map.put locals var head)
-          and-memory m and-trace tr and-rest R
-          and-functions functions)) ->
-      (let head := v in
-       find (cmd.seq (cmd.set
-                        var
-                        (expr.load
-                           access_size.word
-                           (expr.op bopname.add
-                                    (expr.var vector_var)
-                                    (expr.literal ((word.unsigned (word.of_Z 8) * Z.of_nat noffset))))))
-                     k_impl)
-       implementing (pred (dlet head k))
-       with-locals locals and-memory mem and-trace tr and-rest R
-       and-functions functions).
-  Proof.
-    intros.
-    unfold WordVector in *.
-    repeat straightline.
-    exists (word.of_Z (word.unsigned v)).
-    split.
-    { repeat straightline; eauto.
-      exists vector_ptr; intuition.
-      seprewrite_in @array_index_nat_inbounds H0;
-        cycle 1.
-      { eexists.
-        split.
-        { eapply load_word_of_sep.
-          ecancel_assumption. }
-      { subst v.
-        (* FIXME: vector/list lemmas *)
-        admit. } }
-      { rewrite Vector_to_list_length.
-        apply (proj2_sig (Fin.to_nat offset)). } }
-    { repeat straightline.
-      cbv [dlet.dlet].
-      subst l.
-      rewrite word.of_Z_unsigned.
-      eauto. }
-    Unshelve.
-    apply (word.of_Z 0).
-    Admitted.
-
-  Lemma compile_replace :
-    forall (locals: Semantics.locals) (mem: Semantics.mem)
-      tr R R' functions T (pred: T -> _ -> Prop)
-      {n} (vector: Vector.t Semantics.word n) vector_ptr vector_var
-      value value_var offset
-      k k_impl,
-      (Z.of_nat n < 2 ^ Semantics.width)%Z ->
-      sep (WordVector vector_ptr vector) R' mem ->
-      map.get locals vector_var = Some vector_ptr ->
-      map.get locals value_var = Some value ->
-      let v := (Vector.replace vector offset value) in
-      let noffset := proj1_sig (Fin.to_nat offset) in
-      (let head := v in
-       forall m,
-         sep (WordVector vector_ptr head) R' m ->
-         (find k_impl
-          implementing (pred (k head))
-          with-locals locals
-          and-memory m and-trace tr and-rest R
-          and-functions functions)) ->
-      (let head := v in
-       find (cmd.seq (cmd.store access_size.word
-                                (expr.op bopname.add
-                                         (expr.var vector_var)
-                                         (expr.literal ((word.unsigned (word.of_Z 8) * Z.of_nat noffset))))
-                                (expr.var value_var))
-                     k_impl)
-       implementing (pred (dlet head k))
-       with-locals locals and-memory mem and-trace tr and-rest R
-       and-functions functions).
-  Proof.
-    intros.
-    unfold WordVector in *.
-    repeat straightline.
-    exists (word.add vector_ptr
-                     (word.of_Z (word.unsigned (word.of_Z 8) * Z.of_nat noffset))).
-    split.
-    { repeat straightline; eauto.
-      exists vector_ptr; intuition.
-      reflexivity. }
-    { exists value.
+Lemma compile_nth :
+  forall (locals: Semantics.locals) (mem: Semantics.mem)
+    tr R R' functions T (pred: T -> _ -> Prop)
+    {n} (vector: Vector.t Semantics.word n) vector_ptr vector_var
+    offset var k k_impl,
+    (Z.of_nat n < 2 ^ Semantics.width)%Z ->
+    sep (WordVector vector_ptr vector) R' mem ->
+    map.get locals vector_var = Some vector_ptr ->
+    let v := Vector.nth vector offset in
+    let noffset := proj1_sig (Fin.to_nat offset) in
+    (let head := v in
+     forall m,
+       sep (WordVector vector_ptr vector) R' m ->
+       (find k_impl
+        implementing (pred (k head))
+        with-locals (map.put locals var head)
+        and-memory m and-trace tr and-rest R
+        and-functions functions)) ->
+    (let head := v in
+     find (cmd.seq (cmd.set
+                      var
+                      (expr.load
+                         access_size.word
+                         (expr.op bopname.add
+                                  (expr.var vector_var)
+                                  (expr.literal ((word.unsigned (word.of_Z 8) * Z.of_nat noffset))))))
+                   k_impl)
+     implementing (pred (dlet head k))
+     with-locals locals and-memory mem and-trace tr and-rest R
+     and-functions functions).
+Proof.
+  intros.
+  unfold WordVector in *.
+  repeat straightline.
+  exists (word.of_Z (word.unsigned v)).
+  split.
+  { repeat straightline; eauto.
+    exists vector_ptr; intuition.
+    seprewrite_in @array_index_nat_inbounds H0;
+      cycle 1.
+    { eexists.
       split.
-      { straightline.
-        eexists; eauto. }
-      { repeat straightline.
-        eapply store_word_of_sep.
-        { seprewrite_in @array_index_nat_inbounds H0;
-            cycle 1.
-          { ecancel_assumption. }
-          { subst noffset.
-            rewrite Vector_to_list_length.
-            apply (proj2_sig (Fin.to_nat offset)). } }
-        { intros.
-          apply H3.
-          seprewrite (array_index_nat_inbounds (default:=word.of_Z 0) scalar (word.of_Z 8) (Vector.to_list v) vector_ptr (proj1_sig (Fin.to_nat offset))); cycle 1.
-          { admit.                (* Lemmas on Vector.to_list and replace *)
-          }
-          { subst noffset.
-            rewrite Vector_to_list_length.
-            apply (proj2_sig (Fin.to_nat offset)). } }
+      { eapply load_word_of_sep.
+        ecancel_assumption. }
+    { subst v.
+      (* FIXME: vector/list lemmas *)
+      admit. } }
+    { rewrite Vector_to_list_length.
+      apply (proj2_sig (Fin.to_nat offset)). } }
+  { repeat straightline.
+    cbv [dlet.dlet].
+    subst l.
+    rewrite word.of_Z_unsigned.
+    eauto. }
+  Unshelve.
+  apply (word.of_Z 0).
   Admitted.
 
-  Hint Unfold Packet : compiler.
-  Opaque dlet.
+Lemma compile_replace :
+  forall (locals: Semantics.locals) (mem: Semantics.mem)
+    tr R R' functions T (pred: T -> _ -> Prop)
+    {n} (vector: Vector.t Semantics.word n) vector_ptr vector_var
+    value value_var offset
+    k k_impl,
+    (Z.of_nat n < 2 ^ Semantics.width)%Z ->
+    sep (WordVector vector_ptr vector) R' mem ->
+    map.get locals vector_var = Some vector_ptr ->
+    map.get locals value_var = Some value ->
+    let v := (Vector.replace vector offset value) in
+    let noffset := proj1_sig (Fin.to_nat offset) in
+    (let head := v in
+     forall m,
+       sep (WordVector vector_ptr head) R' m ->
+       (find k_impl
+        implementing (pred (k head))
+        with-locals locals
+        and-memory m and-trace tr and-rest R
+        and-functions functions)) ->
+    (let head := v in
+     find (cmd.seq (cmd.store access_size.word
+                              (expr.op bopname.add
+                                       (expr.var vector_var)
+                                       (expr.literal ((word.unsigned (word.of_Z 8) * Z.of_nat noffset))))
+                              (expr.var value_var))
+                   k_impl)
+     implementing (pred (dlet head k))
+     with-locals locals and-memory mem and-trace tr and-rest R
+     and-functions functions).
+Proof.
+  intros.
+  unfold WordVector in *.
+  repeat straightline.
+  exists (word.add vector_ptr
+                   (word.of_Z (word.unsigned (word.of_Z 8) * Z.of_nat noffset))).
+  split.
+  { repeat straightline; eauto.
+    exists vector_ptr; intuition.
+    reflexivity. }
+  { exists value.
+    split.
+    { straightline.
+      eexists; eauto. }
+    { repeat straightline.
+      eapply store_word_of_sep.
+      { seprewrite_in @array_index_nat_inbounds H0;
+          cycle 1.
+        { ecancel_assumption. }
+        { subst noffset.
+          rewrite Vector_to_list_length.
+          apply (proj2_sig (Fin.to_nat offset)). } }
+      { intros.
+        apply H3.
+        seprewrite (array_index_nat_inbounds (default:=word.of_Z 0) scalar (word.of_Z 8) (Vector.to_list v) vector_ptr (proj1_sig (Fin.to_nat offset))); cycle 1.
+        { admit.                (* Lemmas on Vector.to_list and replace *)
+        }
+        { subst noffset.
+          rewrite Vector_to_list_length.
+          apply (proj2_sig (Fin.to_nat offset)). } }
+Admitted.
 
-  Notation "'forall!' x .. y ',' pre '===>' fname '@' args '==>' post" :=
-    (fun functions =>
-       (forall x,
-           .. (forall y,
-                  forall R tr mem,
-                    (pre * R)%sep mem ->
-                    WeakestPrecondition.call
-                      functions fname tr mem args
-                      (postcondition_for post R tr)) ..))
-         (x binder, y binder, only parsing, at level 199).
-  Instance spec_of_decr : spec_of "decr" :=
-    forall! pp p,
-      Packet pp p ===> "decr" @ [pp] ==> Packet pp (decr_gallina p).
+Hint Unfold Packet : compiler.
+Opaque dlet.
 
-  (* TODO: something like program_logic_goal_for_function! *)
-  Derive decr_body SuchThat
-         (let decr := ("decr", (["p"], [], decr_body)) in
-          program_logic_goal_for
-            decr
-            (ltac:(let x := program_logic_goal_for_function decr (@nil string) in
-                   exact x)))
-    As decr_body_correct.
-  Proof.
-    cbv [program_logic_goal_for spec_of_decr].
-    setup.
-    assert (Z.of_nat 2 < 2 ^ Semantics.width)%Z by (cbn; lia).
-    eapply compile_nth with (var := "ttl").
-    1-3:repeat t; eauto.
-    do 6 t.
-    1-2:repeat t.
-    intros.
-    eapply compile_replace.
-    1-4:repeat t; eauto.
-    unfold Packet in *.
-    intros.
-    repeat t.
-  Qed.
-End Ttl.
+Notation "'forall!' x .. y ',' pre '===>' fname '@' args '==>' post" :=
+  (fun functions =>
+     (forall x,
+         .. (forall y,
+                forall R tr mem,
+                  (pre * R)%sep mem ->
+                  WeakestPrecondition.call
+                    functions fname tr mem args
+                    (postcondition_for post R tr)) ..))
+       (x binder, y binder, only parsing, at level 199).
+Instance spec_of_decr : spec_of "decr" :=
+  forall! pp p,
+    Packet pp p ===> "decr" @ [pp] ==> Packet pp (decr_gallina p).
 
+(* TODO: something like program_logic_goal_for_function! *)
+Derive decr_body SuchThat
+       (let decr := ("decr", (["p"], [], decr_body)) in
+        program_logic_goal_for
+          decr
+          (ltac:(let x := program_logic_goal_for_function decr (@nil string) in
+                 exact x)))
+  As decr_body_correct.
+Proof.
+  cbv [program_logic_goal_for spec_of_decr].
+  setup.
+  assert (Z.of_nat 2 < 2 ^ Semantics.width)%Z by (cbn; lia).
+  eapply compile_nth with (var := "ttl").
+  1-3:repeat compile_step; eauto.
+  do 6 compile_step.
+  1-2:repeat compile_step.
+  intros.
+  eapply compile_replace.
+  1-4:repeat compile_step; eauto.
+  repeat compile_step.
+Qed.
