src/Lib/Api.v
@@ -1,0 +1,5 @@
+Require Export Rupicola.Lib.Core.
+Require Export Rupicola.Lib.Tactics.
+Require Export Rupicola.Lib.Notations.
+Require Export Rupicola.Lib.Compiler.
+Require Export Coq.derive.Derive.
