src/Lib/Compiler.v
@@ -1,0 +1,149 @@
+Require Import Rupicola.Lib.Core.
+Require Import Rupicola.Lib.Notations.
+Require Export Rupicola.Lib.Gensym.
+
+Lemma compile_skip :
+  forall (locals: Semantics.locals) (mem: Semantics.mem)
+    tr R functions T (pred: T -> _ -> Prop) head,
+    sep (pred head) R mem ->
+    (find cmd.skip
+     implementing (pred head)
+     with-locals locals and-memory mem and-trace tr and-rest R
+     and-functions functions).
+Proof.
+  intros.
+  repeat straightline.
+  red; red; eauto.
+Qed.
+
+Lemma compile_constant :
+  forall (locals: Semantics.locals) (mem: Semantics.mem)
+    tr R functions T (pred: T -> _ -> Prop) z k k_impl,
+  forall var,
+    let v := word.of_Z z in
+    (let head := v in
+     find k_impl
+     implementing (pred (k head))
+     with-locals (map.put locals var head)
+     and-memory mem and-trace tr and-rest R
+     and-functions functions) ->
+    (let head := v in
+     find (cmd.seq (cmd.set var (expr.literal z)) k_impl)
+     implementing (pred (dlet head k))
+     with-locals locals and-memory mem and-trace tr and-rest R
+     and-functions functions).
+Proof.
+  intros.
+  repeat straightline.
+  eassumption.
+Qed.
+
+(* FIXME add let pattern to other lemmas *)
+Lemma compile_add :
+  forall (locals: Semantics.locals) (mem: Semantics.mem)
+    tr R (* R' *) functions T (pred: T -> _ -> Prop) x x_var y y_var k k_impl,
+  forall var,
+    (* WeakestPrecondition.dexpr mem locals (expr.var x_var) x -> *)
+    (* WeakestPrecondition.dexpr mem locals (expr.var y_var) y -> *)
+    map.get locals x_var = Some x ->
+    map.get locals y_var = Some y ->
+    let v := word.add x y in
+    (let head := v in
+     find k_impl
+     implementing (pred (k head))
+     with-locals (map.put locals var head)
+     and-memory mem and-trace tr and-rest R
+     and-functions functions) ->
+    (let head := v in
+     find (cmd.seq (cmd.set var (expr.op bopname.add (expr.var x_var) (expr.var y_var)))
+                   k_impl)
+     implementing (pred (dlet head k))
+     with-locals locals and-memory mem and-trace tr and-rest R
+     and-functions functions).
+Proof.
+  intros.
+  repeat straightline.
+  eexists; split.
+  { repeat straightline.
+    exists x; split; try eassumption.
+    repeat straightline.
+    exists y; split; try eassumption.
+    reflexivity. }
+  red.
+  eassumption.
+Qed.
+
+Ltac setup_step :=
+  match goal with
+  | _ => progress (cbv zeta; unfold program_logic_goal_for)
+  | [  |- forall _, _ ] => intros
+  | [  |- exists _, _ ] => eexists
+  | [  |- _ /\ _ ] => split
+  | [  |- context[postcondition_for _ _ _] ] =>
+    set (postcondition_for _ _ _)
+  | _ => reflexivity
+  | _ => cbn
+  end.
+
+Ltac term_head x :=
+  match x with
+  | ?f _ => term_head f
+  | _ => x
+  end.
+
+Ltac setup :=
+  repeat setup_step;
+  repeat match goal with
+         | [ H := _ |- _ ] => subst H
+         end;
+  match goal with
+  | [  |- context[postcondition_for (?pred ?spec) ?R ?tr] ] =>
+    change (fun x y _ => postcondition_for (pred spec) R tr x y [])
+      with (postcondition_norets (pred spec) R tr);
+    let hd := term_head spec in
+    unfold hd
+  end.
+
+Ltac lookup_variable locals ptr :=
+  lazymatch locals with
+  | [] => fail
+  | (?k, ptr) :: _ => k
+  | (_, _) :: ?tl => lookup_variable tl ptr
+  end.
+
+Ltac solve_map_get_goal :=
+  lazymatch goal with
+  | [  |- map.get {| value := ?locals; _value_ok := _ |} _ = Some ?val ] =>
+    let var := lookup_variable locals val in
+    instantiate (1 := var);
+    reflexivity
+  end.
+
+Create HintDb compiler.
+
+Ltac compile_basics :=
+  (* FIXME compile_skip applies in all cases, so guard it *)
+  gen_sym_inc;
+  let name := gen_sym_fetch "v" in
+  first [simple eapply compile_constant with (var := name) |
+         simple eapply compile_add with (var := name) |
+         simple eapply compile_skip].
+
+Ltac compile_custom := fail.
+
+Ltac compile_step :=
+  lazymatch goal with
+  | [  |- let _ := _ in _ ] => intros
+  | [  |- context[map.put _ _ _] ] => simpl map.put
+  | [  |- WeakestPrecondition.cmd _ _ _ _ _ _ ] =>
+    first [compile_custom | compile_basics ]
+  | [  |- sep _ _ _ ] =>
+    autounfold with compiler in *;
+    cbn [fst snd] in *;
+    ecancel_assumption
+  | [  |- map.get _ _ = Some _ ] => solve_map_get_goal
+  | _ => eauto with compiler
+  end.
+
+Ltac compile :=
+  setup; repeat compile_step.
