src/Lib/Core.v
@@ -1,0 +1,51 @@
+Require Export Coq.Strings.String.
+Require Export Coq.Lists.List.
+Require Export Coq.ZArith.ZArith.
+Require Export Coq.micromega.Lia.
+Require Export bedrock2.Array.
+Require Export bedrock2.BasicC64Semantics.
+Require Export bedrock2.BasicCSyntax.
+Require Export bedrock2.Map.Separation.
+Require Export bedrock2.ProgramLogic.
+Require Export bedrock2.Map.SeparationLogic.
+Require Export bedrock2.Scalars.
+Require Export bedrock2.Syntax.
+Require Export bedrock2.WeakestPreconditionProperties.
+Require Export coqutil.dlet.
+Require Export coqutil.Map.Interface coqutil.Map.Properties coqutil.Map.SortedList.
+Require Export coqutil.Tactics.Tactics.
+Require Export coqutil.Tactics.letexists.
+Require Export coqutil.Word.Interface coqutil.Word.Properties.
+Require bedrock2.ProgramLogic.
+
+Open Scope string_scope.
+Export ListNotations.
+
+Declare Scope sep_scope.
+Delimit Scope sep_scope with sep.
+Infix "*" := (sep) : sep_scope.
+
+Set Nested Proofs Allowed.
+
+(* TODO: once bedrock2 version is updated, these can be replaced by the
+   commented-out generalized version below. *)
+Local Existing Instance bedrock2.BasicCSyntax.StringNames_params.
+Local Existing Instance BasicC64Semantics.parameters.
+Local Existing Instance BasicC64Semantics.parameters_ok.
+(*
+Context {p : Semantics.parameters} {word_size_in_bytes : Z}.
+Context {p_ok : Semantics.parameters_ok p}.
+ *)
+
+Notation word := Semantics.word.
+
+(* FIXME instead of cbn [fst snd], use simpl never hints in the sep case *)
+Arguments Semantics.word : simpl never.
+
+Notation address := word (only parsing).
+
+Definition bedrock_func : Type :=
+  funname * (list string * list string * cmd).
+Coercion name_of_func (f : bedrock_func) := fst f.
+
+(* FIXME update bedrock2 to get rid of Semantics.byte *)
