src/Lib/Gensym.v
@@ -1,0 +1,20 @@
+Require Import Rupicola.Lib.Core.
+
+Inductive Counter (n : nat) : Type :=
+| ofNat : Counter n
+.
+
+Ltac gen_sym_inc :=
+  lazymatch goal with
+  | H : Counter ?n |- _ =>
+    pose proof (ofNat (S n)); clear H
+  | _ => pose proof (ofNat 0)
+  end.
+
+Ltac gen_sym_fetch prefix :=
+  lazymatch goal with
+  | H : Counter ?n |- _ =>
+    let x := constr:((prefix ++ DecimalString.NilEmpty.string_of_uint (Nat.to_uint n))%string) in
+    let x := eval cbv in x in
+        constr:(x)
+  end.
