src/Lib/LegacyCompiler.v
@@ -1,0 +1,98 @@
+Require Import Rupicola.Lib.Core.
+Require Import Rupicola.Lib.Compiler.
+
+Ltac compile_step := fail.
+
+Ltac match_compile_goal :=
+  lazymatch goal with
+  | [  |- WeakestPrecondition.cmd _ ?b2_body _ ?mem
+                                 {| value := ?locals |}
+                                 (fun (t : Semantics.trace) m _ =>
+                                    _ /\
+                                    _ /\
+                                    sep (_ ?spec) _ m) ] =>
+    compile_step b2_body mem locals spec
+  end.
+
+Ltac lookup_object_in predicates predicate value :=
+  lazymatch predicates with
+  | predicate ?ptr value =>
+    constr:(Some ptr)
+  | sep ?l ?r =>
+    lazymatch lookup_object_in l predicate value with
+    | Some ?ptr => constr:(Some ptr)
+    | None => lookup_object_in r predicate value
+    end
+  | _ => constr:(@None address)
+  end.
+
+Ltac lookup_object predicate value mem :=
+  lazymatch goal with
+  | [ H: ?predicates mem |- _ ] =>
+    let ptr := lookup_object_in predicates predicate value in
+    lazymatch ptr with
+    | Some ?ptr => ptr
+    | None => fail "failed to look up object" value
+    end
+  | _ => fail "failed to find preconditions for " mem
+  end.
+
+Ltac expr_of_constant g :=
+  lazymatch g with
+  | word.of_Z ?z =>
+    constr:(expr.literal z)
+  end.
+
+Ltac expr_of_gallina locals g :=
+  match g with            (* FIXME test with is_var *)
+  | _ => let v := lookup_variable locals g in
+        constr:(expr.var v)
+  | _ => expr_of_constant g
+  | ?other => fail "failed to translate to expr " other
+  end.
+
+Axiom cell_value : Type.
+
+Ltac compile_step b2_body mem locals spec ::=
+  lazymatch spec with
+  | (dlet ?value ?continuation) =>
+    lazymatch value with
+    | get ?c =>
+      let ptr := lookup_object cell_value c mem in
+      let var := expr_of_gallina locals ptr in
+      let b2_continuation := fresh "body" in
+      gen_sym_inc;
+      let name := gen_sym_fetch "v" in
+      evar (b2_continuation: cmd);
+      unify b2_body
+            (cmd.seq (cmd.set name (expr.load access_size.word
+                                              var))
+                     b2_continuation);
+      subst b2_continuation
+    | word.add ?l ?r =>
+      let ll := expr_of_gallina locals l in
+      let rr := expr_of_gallina locals r in
+      gen_sym_inc;
+      let name := gen_sym_fetch "v" in
+      let b2_continuation := fresh "body" in
+      evar (b2_continuation: cmd);
+      unify b2_body (* FIXME coq renamed v into v0 *)
+            (cmd.seq (cmd.set name (expr.op
+                                      bopname.add
+                                      ll rr))
+                     b2_continuation);
+      subst b2_continuation
+    | put ?x ?c =>
+      let ptr := lookup_object cell_value c mem in
+      let var := expr_of_gallina locals ptr in
+      let x := expr_of_gallina locals x in
+      let b2_continuation := fresh "body" in
+      evar (b2_continuation: cmd);
+      unify b2_body
+            (cmd.seq (cmd.store access_size.word var x)
+                     b2_continuation);
+      subst b2_continuation
+    | ?other => fail "Not sure what to do with" other
+    end
+  | _ => unify b2_body (cmd.skip)
+  end.
