src/Lib/Notations.v
@@ -1,0 +1,23 @@
+Require Import Rupicola.Lib.Core.
+
+Notation "'let/d'  x  :=  val  'in'  body" :=
+  (dlet val (fun x => body)) (at level 4).
+
+Infix "~>" := scalar (at level 40, only parsing).
+
+Notation "[[ locals ]]" := ({| value := locals; _value_ok := _ |}) (only printing).
+
+Definition postcondition_for spec R tr :=
+  (fun (tr' : Semantics.trace) (mem' : Semantics.mem) (rets : list address) =>
+     tr = tr' /\ rets = nil
+     /\ sep spec R mem').
+
+Definition postcondition_norets spec R tr :=
+  (fun (tr' : Semantics.trace) (mem' : Semantics.mem) (_ : Semantics.locals) =>
+     postcondition_for spec R tr tr' mem' []).
+
+Notation "'find' body 'implementing' spec 'with-locals' locals 'and-memory' mem 'and-trace' tr 'and-rest' R 'and-functions' fns" :=
+  (WeakestPrecondition.cmd
+     (WeakestPrecondition.call fns)
+     body tr mem locals
+     (postcondition_norets spec R tr)) (at level 0).
