src/Lib/Tactics.v
@@ -1,0 +1,117 @@
+Require Import Rupicola.Lib.Core.
+
+Ltac boolean_cleanup :=
+  repeat match goal with
+         | H : _ |- _ =>
+           rewrite word.unsigned_of_Z_0 in H
+         | H : _ |- _ =>
+           rewrite word.unsigned_of_Z_1 in H
+         | H : ?x = word.of_Z 0%Z |- _ => subst x
+         | H : ?x = word.of_Z 1%Z |- _ => subst x
+         | x := word.of_Z 0%Z |- _ => subst x
+         | x := word.of_Z 1%Z |- _ => subst x
+         | _ => congruence
+         end.
+
+Ltac destruct_lists_of_known_length :=
+  repeat match goal with
+         | H : S _ = S _ |- _ => apply Nat.succ_inj in H
+         | H : length ?x = S _ |- _ =>
+           destruct x; cbn [length] in H; [ congruence | ]
+         | H : length ?x = 0 |- _ =>
+           destruct x; cbn [length] in H; [ clear H | congruence]
+         end;
+  cbn [hd tl] in *.
+
+(* just a wrapper that calls straightline_call + straightline, and also
+   destructs output lists *)
+Ltac handle_call :=
+  ProgramLogic.straightline_call; [ ecancel_assumption | ];
+  repeat ProgramLogic.straightline;
+  destruct_lists_of_known_length;
+  repeat ProgramLogic.straightline.
+
+
+(* stolen from a bedrock2 example file (LAN9250.v) *)
+Ltac split_if :=
+  lazymatch goal with
+    |- WeakestPrecondition.cmd _ ?c _ _ _ ?post =>
+    let c := eval hnf in c in
+        lazymatch c with
+        | Syntax.cmd.cond _ _ _ =>
+          letexists; split;
+          [solve[repeat ProgramLogic.straightline]|split]
+        end
+  end.
+
+Ltac clear_old_seps :=
+  match goal with
+  | H : sep _ _ ?mem |- context [?mem] =>
+    repeat match goal with
+           | H' : sep _ _ ?m |- _ =>
+             assert_fails (unify m mem); clear H'
+           end
+  end.
+
+Ltac cleanup :=
+  repeat first [ progress cbn [fst snd eq_rect] in *
+               | match goal with H : _ /\ _ |- _ => destruct H end
+               | match goal with H : exists _, _ |- _ => destruct H end
+               | match goal with H : ?x = ?x |- _ => clear H end ].
+
+Ltac sepsimpl_step' :=
+  match goal with
+  | |- sep (emp _) _ _ => apply sep_emp_l
+  | |- sep _ (emp _) _ => apply sep_emp_r
+  | |- sep (fun m => emp _ m) _ _ => apply sep_emp_l
+  | |- sep _ (fun m => emp _ m) _ => apply sep_emp_r
+  | |- sep (Lift1Prop.ex1 _) _ _ => apply sep_ex1_l
+  | |- sep _ (Lift1Prop.ex1 _) _ => apply sep_ex1_r
+  | |- emp _ _ => split; [ congruence | ]
+  end.
+
+Ltac sepsimpl_step :=
+  match goal with
+  | _ => sepsimpl_step'
+  | |- sep (sep _ _) _ _ => apply sep_assoc; sepsimpl_step'
+  | |- sep _ (sep _ _) _ => apply sep_comm, sep_assoc; sepsimpl_step'
+  | |- sep _ _ _ => apply sep_comm; sepsimpl_step'
+  end.
+
+Ltac sepsimpl_in H :=
+  match type of H with
+  | sep (emp _) _ _ =>
+    eapply sep_emp_l in H
+  | sep _ (emp _) _ =>
+    eapply sep_emp_r in H
+  | sep (fun m => emp _ m) _ _ =>
+    eapply sep_emp_l in H
+  | sep _ (fun m => emp _ m) _ =>
+    eapply sep_emp_r in H
+  | sep (Lift1Prop.ex1 _) _ _ =>
+    eapply sep_ex1_l in H; destruct H
+  | sep _ (Lift1Prop.ex1 _) _ =>
+    eapply sep_ex1_r in H; destruct H
+  end.
+
+Ltac sepsimpl_hyps_step :=
+  match goal with
+  | H : False |- _ => tauto
+  | H : emp _ _ |- _ => cbv [emp] in H; destruct H
+  | H : Lift1Prop.ex1 _ _ |- _ => destruct H
+  | H : sep (sep ?p ?q) _ _ |- _ =>
+    eapply (sep_assoc p q) in H; sepsimpl_in H
+  | H : sep _ _ _ |- _ => sepsimpl_in H
+  | H : sep _ (sep ?p ?q) _ |- _ =>
+    eapply sep_comm, (sep_assoc p q) in H; sepsimpl_in H
+  end.
+
+Ltac sepsimpl_hyps :=
+  repeat first [ progress cleanup
+               | progress sepsimpl_hyps_step ].
+
+Ltac sepsimpl :=
+  repeat first [ progress cleanup
+               | match goal with |- _ /\ _ => split end
+               | progress sepsimpl_step
+               | progress sepsimpl_hyps_step ].
